CollapsingTowers/TwoLevel/Progresss.lean
@@ -1,15 +1,15 @@
 
 import CollapsingTowers.TwoLevel.Typing
 @[simp]
-def env_wf₁ : TEnv -> Prop
+def env_wfty₁ : TEnv -> Prop
   | [] => true
-  | τ :: τs => wf₁ τ /\ env_wf₁ τs
+  | τ :: τs => wfty₁ τ /\ env_wfty₁ τs
 
-theorem progress𝕔 : ∀ Γ e₀ τ, typing Γ e₀ (.rep τ) -> env_wf₁ Γ -> wf₁ τ -> value e₀ \/ ∃ e₁, step e₀ e₁ :=
+theorem progress𝕔 : ∀ Γ e₀ τ, typing Γ e₀ (.rep τ) -> env_wfty₁ Γ -> wfty₁ τ -> value e₀ \/ ∃ e₁, step e₀ e₁ :=
   by
   intros Γ e₀ τ
   generalize Eqτ : τ.rep = τ𝕔
-  intros Hτ HwfΓ Hwf
+  intros Hτ HwftyΓ Hwfty
   induction Hτ generalizing τ with
   | fvar _ _ _ Hbinds => admit
   | lam𝕔 Γ e _ _ Hτe Hclose IH =>
@@ -17,11 +17,11 @@ theorem progress𝕔 : ∀ Γ e₀ τ, typing Γ e₀ (.rep τ) -> env_wf₁ Γ 
     rw [← close_open_id₀ e Γ.length]
     generalize HEqe : open₀ Γ.length e = e𝕠
     rw [HEqe] at IH Hτe
-    simp at IH Eqτ; rw [Eqτ] at Hwf
-    cases IH Hwf.left HwfΓ Hwf.right with
+    simp at IH Eqτ; rw [Eqτ] at Hwfty
+    cases IH Hwfty.left HwftyΓ Hwfty.right with
     | inl Hvalue => admit
     | inr Hstep => admit
     apply Hclose
   | _ => admit
 
-theorem progress : ∀ e₀ τ, typing [] e₀ τ -> wf τ -> value e₀ \/ ∃ e₁, step e₀ e₁ := by admit
+theorem progress : ∀ e₀ τ, typing [] e₀ τ -> wfty τ -> value e₀ \/ ∃ e₁, step e₀ e₁ := by admit
